Semantic/Fsub/Denotation/Retype.lean
@@ -1,0 +1,84 @@
+import Semantic.Fsub.Denotation.Core
+import Semantic.Fsub.Denotation.Rebind
+namespace Fsub
+
+structure Retype (env1 : TypeEnv s1) (σ : Subst s1 s2) (env2 : TypeEnv s2) where
+  var :
+    ∀ (x : BVar s1 .var),
+      env1.lookup_var x = interp_var env2 (σ.var x)
+
+  tvar :
+    ∀ (X : BVar s1 .tvar),
+      env1.lookup_tvar X ≈ Ty.val_denot env2 (σ.tvar X)
+
+lemma weaken_interp_var {x : Var s} :
+  interp_var env x = interp_var (env.extend_var arg) (x.rename Rename.succ) := by
+  cases x <;> rfl
+
+lemma tweaken_interp_var {x : Var s} :
+  interp_var env x = interp_var (env.extend_tvar d) (x.rename Rename.succ) := by
+  cases x <;> rfl
+
+theorem Retype.liftVar
+  (ρ : Retype env1 σ env2) :
+  Retype (env1.extend_var x) (σ.lift) (env2.extend_var x) where
+  var := fun
+    | .here => rfl
+    | .there y => by
+      conv =>
+        lhs
+        simp [TypeEnv.extend_var, TypeEnv.lookup_var, TypeEnv.lookup]
+      conv =>
+        rhs
+        simp [Subst.lift]
+        simp [<-weaken_interp_var]
+      exact ρ.var y
+  tvar := fun
+    | .there X => by
+      conv =>
+        lhs
+        simp [TypeEnv.extend_var, TypeEnv.lookup_tvar, TypeEnv.lookup]
+      conv =>
+        rhs
+        simp [Subst.lift]
+      apply Denot.equiv_trans _ _ _ (ρ.tvar X)
+      apply weaken_val_denot
+
+theorem Retype.liftTVar
+  (ρ : Retype env1 σ env2) :
+  Retype (env1.extend_tvar d) (σ.lift) (env2.extend_tvar d) where
+  var := fun
+    | .there x => by
+      conv => lhs; simp [TypeEnv.extend_tvar, TypeEnv.lookup_var, TypeEnv.lookup]
+      conv => rhs; simp [Subst.lift, <-tweaken_interp_var]
+      exact ρ.var x
+  tvar := fun
+    | .here => by
+      conv => lhs; simp [TypeEnv.extend_tvar, TypeEnv.lookup_tvar, TypeEnv.lookup]
+      conv =>
+        rhs
+        simp [Subst.lift, Ty.val_denot, TypeEnv.extend_tvar, TypeEnv.lookup_tvar, TypeEnv.lookup]
+      apply Denot.equiv_refl
+    | .there X => by
+      conv =>
+        lhs
+        simp [TypeEnv.extend_tvar, TypeEnv.lookup_tvar, TypeEnv.lookup]
+      conv =>
+        rhs
+        simp [Subst.lift]
+      apply Denot.equiv_trans _ _ _ (ρ.tvar X)
+      apply tweaken_val_denot
+
+mutual
+
+theorem retype_val_denot
+  (ρ : Retype env1 σ env2) :
+  Ty.val_denot env1 T ≈ Ty.val_denot env2 (T.subst σ) := sorry
+
+theorem retype_exp_denot
+  (ρ : Retype env1 σ env2) :
+  Ty.exp_denot env1 T ≈ Ty.exp_denot env2 (T.subst σ) := sorry
+
+end
+
+end Fsub
